compilation/sim_main.cpp
@@ -32,23 +32,23 @@ int main(int argc, char ** argv, char **env) {
       top->RESET = 0;
     top->eval();
 
-    /*
-    std :: cout << "clk: " << main_time / 2 << endl;
+    //std :: cout << "clk: " << main_time / 2 << endl;
 
-    if(top->toHost__024a__024_en == 1)
-      std :: cout << "0: " << top->toHost__024a__024_arg << std :: endl;
+    if(top->CLK == 1) {
+      if(top->toHost__024a__024_en == 1)
+        std :: cout << main_time/2 << " 0: " << top->toHost__024a__024_arg << std :: endl;
 
-    if(top->toHost__024aa__024_en == 1)
-      std :: cout << "1: " << top->toHost__024aa__024_arg << std :: endl;
+      if(top->toHost__024aa__024_en == 1)
+        std :: cout << main_time/2 << " 1: " << top->toHost__024aa__024_arg << std :: endl;
 
-    if(top->toHost__024aaa__024_en == 1)
-      std :: cout << "2: " << top->toHost__024aaa__024_arg << std :: endl;
+      if(top->toHost__024aaa__024_en == 1)
+        std :: cout << main_time/2 << " 2: " << top->toHost__024aaa__024_arg << std :: endl;
 
-    if(top->toHost__024aaaa__024_en == 1)
-      std :: cout << "3: " << top->toHost__024aaaa__024_arg << std :: endl;
-    */
+      if(top->toHost__024aaaa__024_en == 1)
+        std :: cout << main_time/2 << " 3: " << top->toHost__024aaaa__024_arg << std :: endl;
+    }
 
-    tfp->dump(main_time);
+    //tfp->dump(main_time);
 
     main_time++;
   }
