examples/MemCache.v
@@ -1,11 +1,13 @@
 Require Import Ascii Bool String List.
-Require Import Lib.CommonTactics Lib.ilist Lib.Word Lib.Struct.
+Require Import Lib.CommonTactics Lib.ilist Lib.Word Lib.Struct Lib.Indexer.
 Require Import Kami.Syntax Kami.ParametricSyntax Kami.Semantics Kami.Notations Kami.SemFacts.
 Require Import Kami.Wf Kami.Tactics Kami.Specialize Kami.Duplicate Kami.RefinementFacts.
 Require Import Ex.Msi Ex.MemTypes Ex.RegFile Ex.L1Cache Ex.ChildParent Ex.MemDir.
 Require Import Ex.Fifo Ex.NativeFifo Ex.FifoCorrect Kami.ParametricEquiv Kami.ParametricInline Ex.Names.
 
 Set Implicit Arguments.
+
+Definition flattenToMetaModule m := Build_MetaModule (metaModulesRegs m) (metaModulesRules m) (metaModulesMeths m).
 
 Section MemCache.
   Variables IdxBits TagBits LgNumDatas DataBytes: nat.
@@ -15,15 +17,76 @@ Section MemCache.
   Variable LgNumChildren: nat.
 
   Definition l1Cache := getMetaFromSinNat LgNumChildren (l1Cache IdxBits TagBits LgNumDatas DataBytes Id).
+
+  Definition l1cs :=
+    flattenToMetaModule
+      (@getMetaModulesFromRegFile
+         LgNumChildren
+         {| nameVal := cs--dataArray; goodName :=  rfgn cs eq_refl dataArray eq_refl |}
+         ({| nameVal := cs--read0; goodName :=  rfgn cs eq_refl read eq_refl|}
+            ::
+            {| nameVal := cs--read1; goodName :=  rfgn cs eq_refl read eq_refl|}
+            ::
+            {| nameVal := cs--read2; goodName :=  rfgn cs eq_refl read eq_refl|}
+            ::
+            {| nameVal := cs--read3; goodName :=  rfgn cs eq_refl read eq_refl|}
+            ::
+            {| nameVal := cs--read4; goodName :=  rfgn cs eq_refl read eq_refl|}
+            ::
+            {| nameVal := cs--read5; goodName :=  rfgn cs eq_refl read eq_refl|}
+            ::
+            {| nameVal := cs--read6; goodName :=  rfgn cs eq_refl read eq_refl|}
+            ::
+            {| nameVal := cs--read7; goodName :=  rfgn cs eq_refl read eq_refl|}
+            ::
+            {| nameVal := cs--read8; goodName :=  rfgn cs eq_refl read eq_refl|}
+            :: nil)
+         {| nameVal := cs--write; goodName :=  rfgn cs eq_refl write eq_refl|} IdxBits Msi Default).
+  Definition l1tag :=
+    flattenToMetaModule
+      (@getMetaModulesFromRegFile
+         LgNumChildren
+         {| nameVal := tag--dataArray; goodName :=  rfgn tag eq_refl dataArray eq_refl |}
+         ({| nameVal := tag--read0; goodName :=  rfgn tag eq_refl read0 eq_refl |}
+            ::
+            {| nameVal := tag--read1; goodName :=  rfgn tag eq_refl read1 eq_refl |}
+            ::
+            {| nameVal := tag--read2; goodName :=  rfgn tag eq_refl read2 eq_refl |}
+            ::
+            {| nameVal := tag--read3; goodName :=  rfgn tag eq_refl read3 eq_refl |}
+            ::
+            {| nameVal := tag--read4; goodName :=  rfgn tag eq_refl read4 eq_refl |}
+            ::
+            {| nameVal := tag--read5; goodName :=  rfgn tag eq_refl read5 eq_refl |}
+            ::
+            {| nameVal := tag--read6; goodName :=  rfgn tag eq_refl read6 eq_refl |}
+            ::
+            {| nameVal := tag--read7; goodName :=  rfgn tag eq_refl read7 eq_refl |}
+            ::
+            {| nameVal := tag--read8; goodName :=  rfgn tag eq_refl read8 eq_refl |}
+            ::
+            nil)
+         {| nameVal := tag--write; goodName :=  rfgn tag eq_refl write eq_refl |} IdxBits (L1Cache.Tag TagBits) Default).
+  Definition l1line :=
+    flattenToMetaModule
+      (@getMetaModulesFromRegFile
+         LgNumChildren
+         {| nameVal := line--dataArray; goodName :=  rfgn line eq_refl dataArray eq_refl |}
+         ({| nameVal := line--read; goodName :=  rfgn line eq_refl read eq_refl |} :: nil)
+         {| nameVal := line--write; goodName :=  rfgn line eq_refl write eq_refl |} IdxBits
+         (L1Cache.Line LgNumDatas DataBytes) Default).
+
+(*
   Definition l1cs := getMetaFromSinNat LgNumChildren (@regFileS cs%string IdxBits Msi Default eq_refl).
   Definition l1tag :=
     getMetaFromSinNat LgNumChildren (@regFileS tag IdxBits (L1Cache.Tag TagBits) Default eq_refl).
   Definition l1line :=
     getMetaFromSinNat LgNumChildren (@regFileS line IdxBits
                                   (L1Cache.Line LgNumDatas DataBytes) Default eq_refl).
-
+ *)
+  
   Definition l1 := l1Cache +++ (l1cs +++ l1tag +++ l1line).
-
+  
   Definition MIdxBits := IdxBits + TagBits.
 
   Definition fifoRqToP :=
@@ -58,9 +121,37 @@ Section MemCache.
   Definition childParentC := (childParent +++ (fifoRqFromC +++ fifoRsFromC +++ fifoToC))%kami.
 
   Definition memDir := memDir MIdxBits LgNumDatas DataBytes LgNumChildren Id.
+
+  Definition mline :=
+    flattenToMetaModule
+      (@MetaRegFile
+         {| nameVal := mline--dataArray; goodName := rfgn mline eq_refl dataArray eq_refl |}
+         ({| nameVal := mline--read; goodName := rfgn mline eq_refl read eq_refl|} :: nil)
+         {| nameVal := mline--write; goodName := rfgn mline eq_refl write eq_refl |}
+         MIdxBits (MemDir.Line LgNumDatas DataBytes) Default).
+
+  Definition mdir :=
+    flattenToMetaModule
+      (@MetaRegFile
+         {| nameVal := mcs--dataArray; goodName := rfgn mcs eq_refl dataArray eq_refl |}
+         ({| nameVal := mcs--read0; goodName := rfgn mcs eq_refl read0 eq_refl |}
+            ::
+            {| nameVal := mcs--read1; goodName := rfgn mcs eq_refl read1 eq_refl |}
+            ::
+            {| nameVal := mcs--read2; goodName := rfgn mcs eq_refl read2 eq_refl |}
+            ::
+            {| nameVal := mcs--read3; goodName := rfgn mcs eq_refl read3 eq_refl |}
+            ::          
+            nil)
+         {| nameVal := mcs--write; goodName := rfgn mcs eq_refl write eq_refl |}
+         MIdxBits (MemDir.Dir LgNumChildren) Default).
+
+
+  (*
   Definition mline := @regFileM mline MIdxBits (MemDir.Line LgNumDatas DataBytes)
                                 Default eq_refl.
   Definition mdir := @regFileM mcs MIdxBits (MemDir.Dir LgNumChildren) Default eq_refl.
+   *)
 
   Definition memDirC := (memDir +++ mline +++ mdir)%kami.
 
