examples/MemCacheSynth.v
@@ -1,5 +1,5 @@
 Require Import Ascii Bool String List.
-Require Import Lib.CommonTactics Lib.ilist Lib.Word Lib.Struct.
+Require Import Lib.CommonTactics Lib.ilist Lib.Word Lib.Struct Lib.Indexer.
 Require Import Kami.Syntax Kami.ParametricSyntax Kami.Semantics Kami.Notations Kami.SemFacts.
 Require Import Kami.Wf Kami.Tactics Kami.Specialize Kami.Duplicate Kami.RefinementFacts.
 Require Import Ex.Msi Ex.MemTypes Ex.RegFile Ex.L1Cache Ex.ChildParent Ex.MemDir.
@@ -15,6 +15,64 @@ Section MemCache.
   Variable LgNumChildren: nat.
 
   Definition l1Cache1 := getMetaModulesFromSinNat LgNumChildren (l1Cache IdxBits TagBits LgNumDatas DataBytes Id).
+
+
+  Definition l1cs1 :=
+      (@getMetaModulesFromRegFile
+         LgNumChildren
+         {| nameVal := cs--dataArray; goodName :=  rfgn cs eq_refl dataArray eq_refl |}
+         ({| nameVal := cs--read0; goodName :=  rfgn cs eq_refl read eq_refl|}
+            ::
+            {| nameVal := cs--read1; goodName :=  rfgn cs eq_refl read eq_refl|}
+            ::
+            {| nameVal := cs--read2; goodName :=  rfgn cs eq_refl read eq_refl|}
+            ::
+            {| nameVal := cs--read3; goodName :=  rfgn cs eq_refl read eq_refl|}
+            ::
+            {| nameVal := cs--read4; goodName :=  rfgn cs eq_refl read eq_refl|}
+            ::
+            {| nameVal := cs--read5; goodName :=  rfgn cs eq_refl read eq_refl|}
+            ::
+            {| nameVal := cs--read6; goodName :=  rfgn cs eq_refl read eq_refl|}
+            ::
+            {| nameVal := cs--read7; goodName :=  rfgn cs eq_refl read eq_refl|}
+            ::
+            {| nameVal := cs--read8; goodName :=  rfgn cs eq_refl read eq_refl|}
+            :: nil)
+         {| nameVal := cs--write; goodName :=  rfgn cs eq_refl write eq_refl|} IdxBits Msi Default).
+  Definition l1tag1 :=
+      (@getMetaModulesFromRegFile
+         LgNumChildren
+         {| nameVal := tag--dataArray; goodName :=  rfgn tag eq_refl dataArray eq_refl |}
+         ({| nameVal := tag--read0; goodName :=  rfgn tag eq_refl read0 eq_refl |}
+            ::
+            {| nameVal := tag--read1; goodName :=  rfgn tag eq_refl read1 eq_refl |}
+            ::
+            {| nameVal := tag--read2; goodName :=  rfgn tag eq_refl read2 eq_refl |}
+            ::
+            {| nameVal := tag--read3; goodName :=  rfgn tag eq_refl read3 eq_refl |}
+            ::
+            {| nameVal := tag--read4; goodName :=  rfgn tag eq_refl read4 eq_refl |}
+            ::
+            {| nameVal := tag--read5; goodName :=  rfgn tag eq_refl read5 eq_refl |}
+            ::
+            {| nameVal := tag--read6; goodName :=  rfgn tag eq_refl read6 eq_refl |}
+            ::
+            {| nameVal := tag--read7; goodName :=  rfgn tag eq_refl read7 eq_refl |}
+            ::
+            {| nameVal := tag--read8; goodName :=  rfgn tag eq_refl read8 eq_refl |}
+            ::
+            nil)
+         {| nameVal := tag--write; goodName :=  rfgn tag eq_refl write eq_refl |} IdxBits (L1Cache.Tag TagBits) Default).
+  Definition l1line1 :=
+      (@getMetaModulesFromRegFile
+         LgNumChildren
+         {| nameVal := line--dataArray; goodName :=  rfgn line eq_refl dataArray eq_refl |}
+         ({| nameVal := line--read; goodName :=  rfgn line eq_refl read eq_refl |} :: nil)
+         {| nameVal := line--write; goodName :=  rfgn line eq_refl write eq_refl |} IdxBits
+         (L1Cache.Line LgNumDatas DataBytes) Default).
+
+  (*
   Definition l1cs1 := @getMetaModulesFromRegFile LgNumChildren {| nameVal := Indexer.withPrefix cs dataArray;
                                                                  goodName :=  rfgn cs eq_refl dataArray eq_refl |}
                                                {| nameVal := Indexer.withPrefix cs read; goodName :=  rfgn cs eq_refl read eq_refl|}
@@ -29,6 +87,7 @@ Section MemCache.
                               {| nameVal := Indexer.withPrefix line dataArray; goodName :=  rfgn line eq_refl dataArray eq_refl |}
                               {| nameVal := Indexer.withPrefix line read; goodName :=  rfgn line eq_refl read eq_refl |}
                               {| nameVal := Indexer.withPrefix line write; goodName :=  rfgn line eq_refl write eq_refl |} IdxBits (L1Cache.Line LgNumDatas DataBytes) Default.
+   *)
 
   Definition l11 := l1Cache1 ++++ (l1cs1 ++++ l1tag1 ++++ l1line1).
 
@@ -67,6 +126,30 @@ Section MemCache.
 
   Definition memDir1 := memDir MIdxBits LgNumDatas DataBytes LgNumChildren Id.
 
+  Definition mline1 :=
+      (@MetaRegFile
+         {| nameVal := mline--dataArray; goodName := rfgn mline eq_refl dataArray eq_refl |}
+         ({| nameVal := mline--read; goodName := rfgn mline eq_refl read eq_refl|} :: nil)
+         {| nameVal := mline--write; goodName := rfgn mline eq_refl write eq_refl |}
+         MIdxBits (MemDir.Line LgNumDatas DataBytes) Default).
+
+  Definition mdir1 :=
+      (@MetaRegFile
+         {| nameVal := mcs--dataArray; goodName := rfgn mcs eq_refl dataArray eq_refl |}
+         ({| nameVal := mcs--read0; goodName := rfgn mcs eq_refl read0 eq_refl |}
+            ::
+            {| nameVal := mcs--read1; goodName := rfgn mcs eq_refl read1 eq_refl |}
+            ::
+            {| nameVal := mcs--read2; goodName := rfgn mcs eq_refl read2 eq_refl |}
+            ::
+            {| nameVal := mcs--read3; goodName := rfgn mcs eq_refl read3 eq_refl |}
+            ::          
+            nil)
+         {| nameVal := mcs--write; goodName := rfgn mcs eq_refl write eq_refl |}
+         MIdxBits (MemDir.Dir LgNumChildren) Default).
+
+
+  (*
   Definition mline1 := @MetaRegFile
                               {| nameVal := Indexer.withPrefix mline dataArray; goodName := rfgn mline eq_refl dataArray eq_refl |}
                               {| nameVal := Indexer.withPrefix mline read; goodName := rfgn mline eq_refl read eq_refl|}
@@ -76,6 +159,7 @@ Section MemCache.
                               {| nameVal := Indexer.withPrefix mcs dataArray; goodName := rfgn mcs eq_refl dataArray eq_refl |}
                               {| nameVal := Indexer.withPrefix mcs read; goodName := rfgn mcs eq_refl read eq_refl |}
                               {| nameVal := Indexer.withPrefix mcs write; goodName := rfgn mcs eq_refl write eq_refl |} MIdxBits (MemDir.Dir LgNumChildren) Default.
+   *)
 
   Definition memDirC1 := ((MetaMod memDir1) ++++ mline1 ++++ mdir1)%kami.
 
